Execution of a LLBC# program (and not LLBC+).

src/LLBC_sharp_execution.v
@@ -1,4 +1,4 @@
-(** * Mechanized_LLBC.LLBC_sharp_execution : Execution of a LLBC+ program. *)
+(** * Mechanized_LLBC.LLBC_sharp_execution : Execution of LLBC# programs. *)
 From Stdlib Require Import List.
 Import ListNotations.
 From stdpp Require Import decidable pmap.
@@ -96,26 +96,23 @@ Proof.
   exists ty. split; assumption.
 Qed.
 
-(* TODO: rename LLBC_plus_E_Seq_Unit_Propagate to LLBC_plus_E_Seq_Unit_Propagate. *)
-Lemma eval_seq_unit n S0 S1 B2 stmt_l stmt_r
-  (eval_stmt_l : S0 |-{stmt} stmt_l ~>{1 + n} {[rUnit := S1]})
-  (eval_stmt_r : S1 |-{stmt} stmt_r ~>{1 + n} B2) :
-  S0 |-{stmt} (Seq stmt_l stmt_r) ~>{1 + n} B2.
+Lemma eval_seq_unit S0 S1 B2 stmt_l stmt_r
+  (eval_stmt_l : S0 |-# stmt_l ~> {[rUnit := S1]})
+  (eval_stmt_r : S1 |-# stmt_r ~> B2) :
+  S0 |-# (Seq stmt_l stmt_r) ~> B2.
 Proof.
-  eapply LLBC_plus_E_Seq_Unit_Propagate.
+  eapply LLBC_sharp_E_Seq_Unit_Propagate.
   - exact eval_stmt_l.
   - reflexivity.
-  - exact eval_stmt_r.
   - (* TODO: lemma? *)
-    intros r. unfold branching_state. rewrite delete_singleton, lookup_empty.
-    destruct (lookup _ _); constructor.
+    intros r. unfold branching_state. rewrite delete_singleton, lookup_empty. constructor.
+  - exact eval_stmt_r.
 Qed.
 
-Lemma is_join_singletons r S0 S1 Sjoin :
-  leq_symbolic S0 Sjoin -> leq_symbolic S1 Sjoin ->
-  is_join {[r := S0]} {[r := S1]} {[r := Sjoin]}.
+Lemma leq_branching_singleton r Sl Sr :
+  leq_symbolic Sl Sr -> leq_branching {[r := Sl]} {[r := Sr]}.
 Proof.
-  intros ? ? r'. destruct (decide (r' = r)) as [-> | ].
+  intros ? r'. destruct (decide (r' = r)) as [-> | ].
   - simpl_map. constructor; assumption.
   - unfold branching_state. simpl_map. constructor.
 Qed.
@@ -160,7 +157,12 @@ Definition f :=
 Open Scope stdpp.
 (** We execute the function [f] on the most general state. The arguments << x >> and << y >> are initialized as symbolic values, while the local variables are uninitialized. *)
 Definition init_state := {|
-  vars := {[x := LLBC_sharp_symbolic intT; y := LLBC_sharp_symbolic intT; z := bot; cond := bot]};
+  vars := {[
+    x := LLBC_sharp_symbolic intT;
+    y := LLBC_sharp_symbolic intT;
+    z := bot;
+    cond := bot
+  ]};
   anons := empty;
   abstractions := empty;
 |}.
@@ -205,15 +207,15 @@ Section Eval_LLBC_sharp_program.
   Ltac simpl_state :=
     (* We can actually perform vm_compute on sget, because the result is a value and not a state. *)
     repeat (remember (sget _ _ ) eqn:EQN; vm_compute in EQN; subst);
-    compute - [insert alter empty singletonM delete leq_symbolic];
+    compute - [insert alter empty singletonM delete leq_symbolic leq_branching];
     autorewrite with core.
 
-  Lemma safe_f : exists end_state, init_state |-{stmt} f ~>{1} end_state.
+  Lemma safe_f : exists end_state, init_state |-# f ~> end_state.
   Proof.
     eexists.
     eapply eval_seq_unit.
-    (* Evaluation of the computation << x <= y >>. The result is stored in the temporary variable [cond]. *)
-    { eapply LLBC_plus_E_Assign; [ | apply Store with (a := 1%positive)].
+    (** Evaluation of the computation << x <= y >>. The result is stored in the temporary variable [cond]. *)
+    { eapply LLBC_sharp_E_Assign; [ | apply Store with (a := 1%positive)].
       - econstructor.
         + econstructor. eval_var. constructor. constructor. constructor.
         + econstructor. eval_var. constructor. constructor. constructor.
@@ -225,12 +227,13 @@ Section Eval_LLBC_sharp_program.
     }
     simpl_state. eapply eval_seq_unit.
 
-    (* Evaluation of the conditional. *)
-    { eapply LLBC_plus_IfThenElse_Symbolic with (B_join := {[rUnit := join_state]}).
+    (** Evaluation of the conditional. *)
+    { eapply LLBC_sharp_IfThenElse_Symbolic with (B := {[rUnit := join_state]});
+        [ | eapply LLBC_sharp_Weaken_Postcondition..].
       { econstructor. eval_var. constructor. econstructor. constructor. }
 
-      (* Evaluation of the if branch. *)
-      { eapply LLBC_plus_E_Assign; [ | apply Store with (a := 2%positive)].
+      (** Evaluation of the if branch. *)
+      { eapply LLBC_sharp_E_Assign; [ | apply Store with (a := 2%positive)].
         + apply Eval_mut_borrow with (l := lx).
           * eval_var. constructor.
           * compute_done.
@@ -242,28 +245,18 @@ Section Eval_LLBC_sharp_program.
         + apply store_compatible_types_nil.
         + reflexivity. }
 
-      (* Evaluation of the else branch. *)
-      { eapply LLBC_plus_E_Assign; [ | apply Store with (a := 2%positive)].
-        + apply Eval_mut_borrow with (l := ly).
-          * eval_var. constructor.
-          * compute_done.
-          * compute_done.
-          * compute_done.
-          * constructor.
-        + eval_var. constructor.
-        + apply decide_not_contains_outer_loan_correct. constructor.
-        + apply store_compatible_types_nil.
-        + reflexivity. }
-
-      apply is_join_singletons.
-      (* The state [S_join] is more abstract than the state at the end of the if branch. *)
-      { simpl_state.
+      (** The state [join_state] is more abstract than the state at the end of the if branch. *)
+      { simpl_state. apply leq_branching_singleton.
         eapply prove_leq_symbolic.
-        { eapply Leq_Reborrow_MutBorrow_Abs with (sp := (encode_var z, [])) (l1 := lz) (i := 1%positive) (kb := 1%positive) (kl := 3%positive); try compute_done.
+        { eapply Leq_Reborrow_MutBorrow_Abs
+            with (sp := (encode_var z, [])) (l1 := lz) (i := 1%positive)
+                 (kb := 1%positive) (kl := 3%positive);
+            try compute_done.
           eapply var_not_in_abstraction; reflexivity. reflexivity. constructor. }
         simpl_state.
         eapply prove_leq_symbolic.
-        { eapply Leq_Fresh_MutLoan_Abs with (sp := (encode_var y, [])) (l' := ly) (i := 2%positive) (k := 2%positive);
+        { eapply Leq_Fresh_MutLoan_Abs
+            with (sp := (encode_var y, [])) (l' := ly) (i := 2%positive) (k := 2%positive);
             [compute_done | now eapply var_not_in_abstraction | compute_done.. | constructor]. }
         simpl_state.
         eapply prove_leq_symbolic; [constructor | ].
@@ -282,13 +275,31 @@ Section Eval_LLBC_sharp_program.
         { remove_anon 2%positive. apply Leq_RemoveAnon. all: compute_done. }
         reflexivity. }
 
-      (* The state [S_join] is more abstract than the state at the end of the else branch. *)
-      { eapply prove_leq_symbolic.
-        { eapply Leq_Reborrow_MutBorrow_Abs with (sp := (encode_var z, [])) (l1 := lz) (i := 1%positive) (kb := 2%positive) (kl := 3%positive); try compute_done.
+      (** Evaluation of the else branch. *)
+      { eapply LLBC_sharp_E_Assign; [ | apply Store with (a := 2%positive)].
+        + apply Eval_mut_borrow with (l := ly).
+          * eval_var. constructor.
+          * compute_done.
+          * compute_done.
+          * compute_done.
+          * constructor.
+        + eval_var. constructor.
+        + apply decide_not_contains_outer_loan_correct. constructor.
+        + apply store_compatible_types_nil.
+        + reflexivity. }
+
+      (** The state [join_state] is more abstract than the state at the end of the else branch. *)
+      { simpl_state. apply leq_branching_singleton.
+        eapply prove_leq_symbolic.
+        { eapply Leq_Reborrow_MutBorrow_Abs
+            with (sp := (encode_var z, [])) (l1 := lz) (i := 1%positive)
+                        (kb := 2%positive) (kl := 3%positive);
+            try compute_done.
           eapply var_not_in_abstraction; reflexivity. reflexivity. constructor. }
         simpl_state.
         eapply prove_leq_symbolic.
-        { eapply Leq_Fresh_MutLoan_Abs with (sp := (encode_var x, [])) (l' := lx) (i := 2%positive) (k := 1%positive);
+        { eapply Leq_Fresh_MutLoan_Abs
+            with (sp := (encode_var x, [])) (l' := lx) (i := 2%positive) (k := 1%positive);
             [compute_done | now eapply var_not_in_abstraction | compute_done.. | constructor]. }
         simpl_state.
         eapply prove_leq_symbolic; [constructor | ].
@@ -311,7 +322,7 @@ Section Eval_LLBC_sharp_program.
 
     (* Execution of the line << *z += 1 >> *)
     eapply eval_seq_unit.
-    { eapply LLBC_plus_E_Assign; [ | apply Store with (a := 1%positive)].
+    { eapply LLBC_sharp_E_Assign; [ | apply Store with (a := 1%positive)].
       - econstructor.
         + eapply Eval_copy.
           * eval_var. repeat econstructor || easy.
@@ -325,10 +336,10 @@ Section Eval_LLBC_sharp_program.
     }
     simpl_state.
 
-    (* In order to access the variable << x >>, we must perform reorganizations in order to end the loan [lx.] *)
-    eapply LLBC_plus_E_Reorg.
+    (** In order to access the variable << x >>, we must perform reorganizations in order to end the loan [lx.] *)
+    eapply LLBC_sharp_E_Reorg.
     { etransitivity.
-      (* Ending the loan [lz] ... *)
+      (** Ending the loan [lz] ... *)
       { constructor.
         eapply Reorg_end_borrow_m_in_abstraction
           with (i' := 1%positive) (j' := 3%positive) (q := (encode_var 3%positive, [])).
@@ -339,7 +350,7 @@ Section Eval_LLBC_sharp_program.
         - intros ? ?. apply not_strict_prefix_nil.
         - eapply var_not_in_abstraction. reflexivity. }
       simpl_state. etransitivity.
-      (* ... so that we could end the region abstraction ... *)
+      (** ... so that we could end the region abstraction ... *)
       { constructor.
         remove_abstraction 1%positive. apply Reorg_end_abstraction.
         - reflexivity.
@@ -349,7 +360,7 @@ Section Eval_LLBC_sharp_program.
           apply UnionEmpty.
       }
       simpl_state.
-      (* ... so that we could end the loan [lx]. *)
+      (** ... so that we could end the loan [lx]. *)
       { constructor.
         eapply Reorg_end_borrow_m with (p := (encode_var 1%positive, []))
                                        (q := (encode_anon 2%positive, [])).
@@ -364,8 +375,8 @@ Section Eval_LLBC_sharp_program.
     }
     simpl_state.
 
-    (* Execution of the line << x += 2 >> *)
-    eapply LLBC_plus_E_Assign; [ | apply Store with (a := 5%positive)].
+    (** Execution of the line << x += 2 >> *)
+    eapply LLBC_sharp_E_Assign; [ | apply Store with (a := 5%positive)].
     - econstructor.
       + eapply Eval_copy; [eval_var | ]; constructor. constructor.
       + constructor.
